steel/formats/lowstar/Zeta.LowStar.LogEntry.fsti
@@ -5,3 +5,5 @@ open Zeta.LowStar.Parser
 val parser_log_entry : parser spec_parser_log_entry
 
 val serialize_stamped_record : serializer spec_serializer_stamped_record
+
+val serialize_value : serializer spec_serializer_value
