steel/formats/spec/Zeta.Formats.Synth.fsti
@@ -15,3 +15,17 @@ val synth_record_injective
 
 val synth_record_inverse
 : squash (LPC.synth_inverse synth_record synth_record_recip)
+
+val synth_value
+  (x: Zeta.Formats.Aux.Value.value)
+: Tot Zeta.Steel.LogEntry.Types.value
+
+val synth_value_recip
+  (x: Zeta.Steel.LogEntry.Types.value)
+: Tot Zeta.Formats.Aux.Value.value
+
+val synth_value_injective
+: squash (LPC.synth_injective synth_value)
+
+val synth_value_inverse
+: squash (LPC.synth_inverse synth_value synth_value_recip)
